lambda2Gmu/Preservation.v
@@ -12,28 +12,54 @@ Qed.
 
 Hint Resolve okt_is_ok.
 
-Lemma wft_weakening : forall Σ E F G T,
+Lemma wft_weaken : forall Σ E F G T,
     wft Σ (E & G) T ->
-    okt Σ (E & F & G) ->
+    ok (E & F & G) ->
     wft Σ (E & F & G) T.
-  introv.
-  generalize E F G.
-  induction T; intros; eauto;
-    inversion H; subst.
-  - econstructor; apply* binds_weaken.
-  - econstructor.
-    + eapply IHT1 in H5; eauto.
-    + eapply IHT2 in H6; eauto.
-  - econstructor.
-    + eapply IHT1 in H5; eauto.
-    + eapply IHT2 in H6; eauto.
-  - econstructor.
-    introv.
-    intros HXiL.
-    lets H_: (H4 X HXiL).
-    (* lets H__: (IHT E0 F0 (G0 & X ~ bind_typ)). *)
-    inversion H_; subst; eauto.
-    admit.
+  intros. gen_eq K: (E & G). gen E F G.
+  induction H; intros; subst; auto.
+  (* case: var *)
+  apply (@wft_var Σ (E0 & F & G) X).  apply* binds_weaken.
+  (* case: all *)
+  apply_fresh* wft_all as X. apply_ih_bind* H0.
+Qed.
+
+Lemma wft_strengthen : forall Σ E F x U T,
+ wft Σ (E & (x ~: U) & F) T -> wft Σ (E & F) T.
+Proof.
+  intros. gen_eq G: (E & (x ~: U) & F). gen F.
+  induction H; intros F EQ; subst; auto.
+  apply* (@wft_var).
+  destruct (binds_concat_inv H) as [?|[? ?]].
+    apply~ binds_concat_right.
+    destruct (binds_push_inv H1) as [[? ?]|[? ?]].
+      subst. false.
+      apply~ binds_concat_left.
+  (* todo: binds_cases tactic *)
+  apply_fresh* wft_all as Y. apply_ih_bind* H0.
+Qed.
+
+(** ** Environment is unchanged by substitution from a fresh name *)
+
+Lemma notin_fv_tt_open : forall Y X T,
+  X \notin fv_typ (T open_tt_var Y) ->
+  X \notin fv_typ T.
+Proof.
+ introv. unfold open_tt. generalize 0.
+ induction T; simpl; intros k Fr; auto.
+ specializes IHT1 k. specializes IHT2 k. auto.
+ specializes IHT1 k. specializes IHT2 k. auto.
+ eauto.
+Qed.
+
+Lemma notin_fv_wf : forall Σ E X T,
+  wft Σ E T -> X # E -> X \notin fv_typ T.
+Proof.
+  induction 1; intros Fr; simpl.
+  eauto.
+  rewrite notin_singleton. intro. subst. applys binds_fresh_inv H Fr.
+  notin_simpl; auto.
+  notin_simpl; auto. pick_fresh Y. apply* (@notin_fv_tt_open Y).
 Qed.
 
 Lemma typing_weakening : forall Σ E F G e T,
@@ -41,12 +67,29 @@ Lemma typing_weakening : forall Σ E F G e T,
    okt Σ (E & F & G) ->
    {Σ, E & F & G} ⊢ e ∈ T.
 Proof.
-  introv Typ. gen F. inductions Typ; introv Ok; eauto.
-  apply* typing_var. apply* binds_weaken.
-  apply_fresh* typing_abs as x.
-  admit.
-  forwards~ K: (H0 x).
-Admitted.
+  introv HTyp. gen F. inductions HTyp; introv Ok; eauto.
+  - apply* typing_var. apply* binds_weaken.
+  - apply_fresh* typing_abs as x. apply* wft_weaken.
+    forwards~ K: (H0 x).
+    apply_ih_bind (H1 x); eauto.
+    econstructor; eauto.
+    apply* wft_weaken.
+  - apply_fresh* typing_tabs as X.
+    forwards~ K: (H0 X).
+    apply_ih_bind (H1 X).
+    eauto. auto.
+    econstructor; eauto.
+  - apply* typing_tapp. apply* wft_weaken.
+  - apply_fresh typing_let as x.
+    apply wft_weaken. exact H.
+    eauto.
+    eauto.
+    intros.
+    forwards~ K: (H0 x); eauto.
+    apply_ih_bind (H1 x); eauto.
+    econstructor; eauto.
+    apply* wft_weaken.
+Qed.
 
 Lemma typing_through_subst_ee : forall Σ E F x u U e T,
     {Σ, E & (x ~: T) & F} ⊢ e ∈ T ->
